dafny/concrete-interpreter/Helpers.dfy
@@ -1,0 +1,15 @@
+include "BoundedInts.dfy"
+include "Types.dfy"
+
+module Helpers {
+    import opened BoundedInts
+    import opened Types
+
+    // Assumption: Giving the default value as zero if not present in the map
+    // TODO: Confirm the assumption
+    function getRegValue(reg: Register, values: RegisterMap): RegisterValue
+    {
+        if reg in values then values[reg]
+        else 0
+    }
+}
